theories/Handlers/KV.v
@@ -1,0 +1,78 @@
+From LibTx Require Import
+     SLOT
+     EqDec
+     Storage.
+
+(** Reliable key-value storage IO handler *)
+(* Record KV : Type := *)
+(*   makeKV *)
+(*     { key_t : Set; *)
+(*       val_t : Set; *)
+(*       backend : Set; *)
+(*       key_eq_dec : EqDec key_t; *)
+(*       store_t : @Storage key_t val_t backend; *)
+(*     }.  *)
+
+Section defn.
+  Context {PID K V : Set} {S : Set} `{HStore : @Storage K V S} `{HKeq_dec : EqDec K}.
+
+  (* Context {PID : Set} {kv : KV}. *)
+  (* Let K := key_t kv. *)
+  (* Let V := val_t kv. *)
+  (* Let S := backend kv. *)
+  (* Let HStore := store_t kv. *)
+
+  Inductive req_t :=
+  | read : K -> req_t
+  | delete : K -> req_t
+  | write : K -> V -> req_t
+  | snapshot : req_t.
+
+  Definition ret_t (req : req_t) : Set :=
+    match req with
+    | read _ => option V
+    | delete _ => True
+    | write _ _ => True
+    | snapshot => S
+    end.
+
+  Let ctx := mkCtx PID req_t ret_t.
+  Let TE := @TraceElem ctx.
+
+  Inductive kv_chain_rule : S -> S -> TE -> Prop :=
+  | kv_read : forall pid s k,
+      kv_chain_rule s s (trace_elem ctx pid (read k) (get k s))
+  | kv_write : forall pid s k v,
+      kv_chain_rule s (put k v s) (trace_elem ctx pid (write k v) I)
+  | kv_delete : forall pid s k,
+      kv_chain_rule s (Storage.delete k s) (trace_elem ctx pid (delete k) I)
+  | kv_snapshot : forall pid s,
+      kv_chain_rule s s (trace_elem ctx pid snapshot s).
+
+  Definition t : t :=
+    {| h_state := S;
+       h_req := req_t;
+       h_initial_state := fun x => x = Storage.new;
+       h_chain_rule := kv_chain_rule;
+    |}.
+End defn.
+
+Section Properties.
+  Context {PID K V : Set} {S : Set} `{HStore : @Storage K V S} `{HKeq_dec : EqDec K}.
+
+  Let ctx := mkCtx PID (@req_t K V) (@ret_t K V S).
+  Let TE := @TraceElem ctx.
+
+  Notation "pid '@' ret '<~' req" := (@trace_elem ctx pid req ret).
+
+  Inductive KvTEComm : TE -> TE -> Prop :=
+  | kv_rr_comm : forall p1 p2 k1 k2 v1 v2,
+      KvTEComm (p1 @ v1 <~ read k1)
+               (p2 @ v2 <~ read k2)
+  | kv_rs_comm : forall p1 p2 k v s,
+      KvTEComm (p1 @ v <~ read k)
+               (p2 @ s <~ snapshot).
+
+  Fail Lemma kv_comm : forall te1 te2, KvTEComm te1 te2 <->
+                             @trace_elems_commute S TE _ te1 te2.
+End Properties.
