theories/Handlers/Mutable.v
@@ -1,0 +1,42 @@
+From Coq Require Import
+     List.
+
+Import ListNotations.
+
+From LibTx Require Import
+     SLOT.EventTrace
+     SLOT.Handler.
+
+Inductive req_t {T : Set} :=
+| get : req_t
+| put : T -> req_t.
+
+Section defs.
+  Context (PID T : Set) (initial_state : T -> Prop).
+
+  Local Definition ret_t (req : @req_t T) : Set :=
+    match req with
+    | get => T
+    | _   => True
+    end.
+
+  Let ctx := mkCtx PID req_t ret_t.
+  Let TE := @TraceElem ctx.
+
+  Inductive mut_chain_rule : T -> T -> TE -> Prop :=
+  | mut_get : forall s pid,
+      mut_chain_rule s s (trace_elem ctx pid get s)
+  | mut_put : forall s val pid,
+      mut_chain_rule s val (trace_elem ctx pid (put val) I).
+
+  Definition t : t :=
+    {|
+      h_state := T;
+      h_req := req_t;
+      h_initial_state := initial_state;
+      h_chain_rule := mut_chain_rule;
+    |}.
+
+  Fail Lemma mut_get_comm : forall v pid1 pid2, (*TODO*)
+      trace_elems_commute (trace_elem ctx pid1 get v) (trace_elem ctx pid2 get v).
+End defs.
