theories/Handlers/Mutex.v
@@ -1,0 +1,74 @@
+From Coq Require Import
+     List.
+
+Import ListNotations.
+
+From LibTx Require Import
+     SLOT.EventTrace
+     SLOT.Hoare
+     SLOT.Handler.
+
+Section defs.
+  Open Scope hoare_scope.
+  Inductive req_t : Set :=
+  | grab    : req_t
+  | release : req_t.
+
+  Local Definition ret_t (req : req_t) : Set :=
+    match req with
+    | grab => True
+    | release => bool
+    end.
+
+  Variable PID : Set.
+
+  Definition state_t : Set := option PID.
+
+  Let ctx := mkCtx PID req_t ret_t.
+  Let TE := @TraceElem ctx.
+
+  Inductive mutex_chain_rule : state_t -> state_t -> TE -> Prop :=
+  | mutex_grab : forall pid,
+      mutex_chain_rule None (Some pid) (trace_elem ctx pid grab I)
+  | mutex_release_ok : forall pid,
+      mutex_chain_rule (Some pid) None (trace_elem ctx pid release true)
+  | mutex_release_fail : forall pid,
+      mutex_chain_rule (Some pid) None (trace_elem ctx pid release false).
+
+  Definition t : t :=
+    {|
+      h_state         := state_t;
+      h_req           := req_t;
+      h_initial_state := fun s0 => s0 = None;
+      h_chain_rule    := mutex_chain_rule
+    |}.
+
+  Notation "pid '@' ret '<~' req" := (@trace_elem ctx pid req ret).
+
+  Theorem no_double_grab_0 : forall (a1 a2 : PID),
+      ~(@PossibleTrace PID t [a1 @ I <~ grab;
+                              a2 @ I <~ grab]).
+  Proof.
+    intros a1 a2 H.
+    destruct H as [s [s' H]].
+    inversion_ H.
+    inversion_ H3.
+    inversion_ H5.
+    inversion_ H4.
+  Qed.
+
+  Let state_space := state_t. Let trace_elem := req_t.
+
+  Theorem no_double_grab : forall (a1 a2 : PID),
+      {{ fun (_ : h_state t) => True }}
+        [a1 @ I <~ grab;
+         a2 @ I <~ grab]
+      {{ fun _ => False}}.
+  Proof.
+    intros a1 a2 s s' Hss' Hpre.
+    inversion_ Hss'.
+    inversion_ H2.
+    inversion_ H4.
+    inversion_ H3.
+  Qed.
+End defs.
